---
metadata:
    description: In this twitter proof I show how to maximise the product of two terms whose sum is fixed.
title: 'Twitter proof: maximising the product with a fixed sum'
---

Let's prove that if you want to maximise $ab$ with $a + b$ equal to a constant value $k$, then you want $a = b = \frac{k}{2}$.

===

![maximising ab with a+b=k is achieved with a=b=k/2](max.png)

### Twitter proof

Take $s = k/2$. If $a = s+h$ then $b = s-h$, from which $ab = (s+h)(s-h) = s^2 - h^2$. $h^2 \geq 0$ so $ab$ is maximised when $h = 0$, that is $a = b = s = k/2$.



Do you have an idea for a twitter proof? Let me know in the comments below!
